spec/vfmConstantsScript.sml
@@ -1,0 +1,110 @@
+open HolKernel boolLib bossLib Parse
+
+val () = new_theory "vfmConstants";
+
+Definition stack_limit_def[simp]:
+  stack_limit = 1024n
+End
+
+Definition context_limit_def[simp]:
+  context_limit = 1024n
+End
+
+Definition base_cost_def:
+  base_cost = 21000n
+End
+
+Definition create_cost_def:
+  create_cost = 32000n
+End
+
+Definition call_data_cost_def:
+  call_data_cost is_zero =
+  if is_zero then 4n else 16
+End
+
+Definition init_code_word_cost_def:
+  init_code_word_cost = 2n
+End
+
+Definition code_deposit_cost_def:
+  code_deposit_cost = 200n
+End
+
+Definition warm_access_cost_def:
+  warm_access_cost = 100n
+End
+
+Definition cold_sload_cost_def:
+  cold_sload_cost = 2100n
+End
+
+Definition cold_access_cost_def:
+  cold_access_cost = 2600n
+End
+
+Definition memory_cost_per_word_def:
+  memory_cost_per_word = 3n
+End
+
+Definition memory_copy_cost_def:
+  memory_copy_cost = 3n
+End
+
+Definition exp_per_byte_cost_def:
+  exp_per_byte_cost = 50n
+End
+
+Definition keccak256_per_word_cost_def:
+  keccak256_per_word_cost = 6n
+End
+
+Definition storage_set_cost_def:
+  storage_set_cost = 20000n
+End
+
+Definition storage_update_cost_def:
+  storage_update_cost = 5000n
+End
+
+Definition storage_clear_refund_def:
+  storage_clear_refund = 4800n
+End
+
+Definition log_topic_cost_def:
+  log_topic_cost = 375n
+End
+
+Definition log_data_cost_def:
+  log_data_cost = 8n
+End
+
+Definition new_account_cost_def:
+  new_account_cost = 25000n
+End
+
+Definition call_value_cost_def:
+  call_value_cost = 9000n
+End
+
+Definition self_destruct_new_account_cost_def:
+  self_destruct_new_account_cost = 25000n
+End
+
+Definition call_stipend_def:
+  call_stipend = 2300n
+End
+
+Definition word_size_def:
+  word_size byteSize = (byteSize + 31) DIV 32
+End
+
+Definition access_list_address_cost_def:
+  access_list_address_cost = 2400n
+End
+
+Definition access_list_storage_key_cost_def:
+  access_list_storage_key_cost = 1900n
+End
+
+val () = export_theory();
